Fully-featured bit-list Haskell package

opentheory/theories/all.ml
@@ -49,7 +49,6 @@ loads "opentheory/theories/natural-bits/natural-bits.ml";;
 (* The divides relation on natural numbers.                                  *)
 (* ------------------------------------------------------------------------- *)
 
-(***
 loads "opentheory/theories/natural-divides/natural-divides.ml";;
 
 (* ------------------------------------------------------------------------- *)
@@ -214,5 +213,4 @@ loads "opentheory/theories/haskell-char/haskell-char.ml";;
 (* ------------------------------------------------------------------------- *)
 
 loads "opentheory/theories/haskell-prime/haskell-prime.ml";;
-***)
 ***)
